src/TrsSim.v
@@ -1,6 +1,6 @@
 Require Import Bool List String Peano_dec.
-Require Import Common FMap Syntax Semantics StepDet SemFacts.
-Require Import Simulation Serial.
+Require Import Common FMap ListSupport Syntax Semantics StepDet SemFacts.
+Require Import Simulation Serial SerialFacts.
 
 Require Import Omega.
 
@@ -85,4 +85,331 @@ Section TrsSim.
   Qed.
 
 End TrsSim.
+
+Section MTypePreserving.
+
+  Definition mtPreservingPMsg (pmsg: PMsg) :=
+    forall pre val,
+      Forall (fun mout => mid_type (msg_id mout) = mid_type (pmsg_mid pmsg))
+             (pmsg_outs pmsg pre val).
+
+  Definition mtPreservingObj (obj: Object) :=
+    Forall mtPreservingPMsg (obj_trs obj).
+
+  Definition mtPreservingObs (obs: list Object) :=
+    Forall mtPreservingObj obs.
+
+  Definition mtPreservingSys (sys: System) :=
+    mtPreservingObs (sys_objs sys).
+
+End MTypePreserving.
+
+Section MTypeDisj.
+
+  Definition MTypeDisj (pmsgs1 pmsgs2: list PMsg) :=
+    forall pmsg1 pmsg2,
+      In pmsg1 pmsgs1 ->
+      In pmsg2 pmsgs2 ->
+      mid_type (pmsg_mid pmsg1) <> mid_type (pmsg_mid pmsg2).
+
+  Definition MTypeDisjSys (sys1 sys2: System) :=
+    MTypeDisj (pmsgsOf sys1) (pmsgsOf sys2).
+
+  Lemma MTypeDisj_sym:
+    forall ms1 ms2,
+      MTypeDisj ms1 ms2 ->
+      MTypeDisj ms2 ms1.
+  Proof.
+    unfold MTypeDisj; intros; firstorder.
+  Qed.
+
+  Lemma MTypeDisj_SubList_1:
+    forall ms1 ms2,
+      MTypeDisj ms1 ms2 ->
+      forall ms3,
+        SubList ms3 ms1 ->
+        MTypeDisj ms3 ms2.
+  Proof.
+    unfold MTypeDisj; intros; auto.
+  Qed.
+
+  Lemma MTypeDisj_SubList_2:
+    forall ms1 ms2,
+      MTypeDisj ms1 ms2 ->
+      forall ms3,
+        SubList ms3 ms2 ->
+        MTypeDisj ms1 ms3.
+  Proof.
+    unfold MTypeDisj; intros; auto.
+  Qed.
+
+End MTypeDisj.
+
+Lemma mtPreservineSys_atomic_same_msg_type:
+  forall sys,
+    mtPreservingSys sys ->
+    forall tid min mty hst mouts,
+      Atomic sys tid min hst mouts ->
+      mty = mid_type (msg_id (tmsg_msg min)) ->
+      forall ist1 ist2,
+        steps_det sys ist1 hst ist2 ->
+        Forall (fun msg => mid_type (msg_id (tmsg_msg msg)) = mty) mouts /\
+        Forall (fun tl =>
+                  match tl with
+                  | IlblIn msg => mid_type (msg_id (tmsg_msg msg)) = mty
+                  | IlblOuts (Some hdl) _ => mid_type (msg_id (tmsg_msg hdl)) = mty
+                  | IlblOuts None _ => True
+                  end) hst.
+Proof.
+  induction 2; simpl; intros; [split; repeat constructor; auto|].
+
+  inv H3.
+  specialize (IHAtomic eq_refl _ _ H7); dest.
+  split.
+  - apply Forall_app.
+    + apply Forall_remove; assumption.
+    + eapply Forall_forall in H2; eauto.
+      rewrite <-H2.
+
+      (* NOTE: extract as a lemma? *)
+      clear -H H9.
+      inv H9.
+      * unfold mtPreservingSys, mtPreservingObs in H.
+        eapply Forall_forall in H; eauto.
+        unfold mtPreservingObj in H.
+        eapply Forall_forall in H; eauto.
+        unfold mtPreservingPMsg in H.
+        clear -H H10.
+        specialize (H os (msg_value (getMsg fmsg))).
+        induction (pmsg_outs fpmsg os (msg_value (getMsg fmsg))); [constructor|].
+        simpl in *.
+        inv H; constructor; auto.
+        simpl; rewrite H10, H2.
+        reflexivity.
+      * unfold mtPreservingSys, mtPreservingObs in H.
+        eapply Forall_forall in H; eauto.
+        unfold mtPreservingObj in H.
+        eapply Forall_forall in H; eauto.
+        unfold mtPreservingPMsg in H.
+        clear -H H10.
+        specialize (H os (msg_value (getMsg hdl))).
+        induction (pmsg_outs fpmsg os (msg_value (getMsg hdl))); [constructor|].
+        simpl in *.
+        inv H; constructor; auto.
+        simpl; rewrite H10, H2.
+        reflexivity.
+      
+  - constructor; auto.
+    eapply Forall_forall in H2; eauto.
+Qed.
+
+Section Compositionality.
+
+  Variables (impl1 impl2 spec: System)
+            (simR: TState -> TState -> Prop)
+            (simP: Label -> Label).
+
+  Local Infix "≈" := simR (at level 30).
+
+  Hypotheses (Hidx: indicesOf impl1 = indicesOf impl2)
+             (Hmt1: mtPreservingSys impl1)
+             (Hmt2: mtPreservingSys impl2)
+             (Hmtdisj: MTypeDisjSys impl1 impl2)
+             (Hsim1: TrsSimulates simR simP impl1 spec)
+             (Hsim2: TrsSimulates simR simP impl2 spec).
+
+  Variable (impl: System).
+  Hypotheses (Hmt: mtPreservingSys impl)
+             (Hii: indicesOf impl = indicesOf impl1)
+             (Himpl:
+                forall pmsg iobj,
+                  In pmsg (obj_trs iobj) ->
+                  In iobj (sys_objs impl) ->
+                  exists obj,
+                    obj_idx obj = obj_idx iobj /\
+                    In pmsg (obj_trs obj) /\
+                    In obj (sys_objs impl1 ++ sys_objs impl2)).
+
+  Lemma MTypeDisjSys_distr_same_type:
+    forall mty,
+      (forall pmsg,
+          mid_type (pmsg_mid pmsg) = mty ->
+          forall iobj,
+            In pmsg (obj_trs iobj) -> In iobj (sys_objs impl) ->
+            exists obj : Object,
+              obj_idx obj = obj_idx iobj /\ In pmsg (obj_trs obj) /\
+              In obj (sys_objs impl1)) \/
+      (forall pmsg,
+          mid_type (pmsg_mid pmsg) = mty ->
+          forall iobj,
+            In pmsg (obj_trs iobj) -> In iobj (sys_objs impl) ->
+            exists obj : Object,
+              obj_idx obj = obj_idx iobj /\ In pmsg (obj_trs obj) /\
+              In obj (sys_objs impl2)).
+  Proof.
+    intros.
+    destruct (mty ?<n (map (fun pmsg => mid_type (pmsg_mid pmsg)) (pmsgsOf impl1))).
+    - left; intros.
+      pose proof (Himpl _ _ H0 H1).
+      destruct H2 as [obj [? [? ?]]].
+      apply in_app_or in H4; destruct H4.
+      + exists obj; repeat split; assumption.
+      + exfalso.
+        pose proof (pmsgsOf_in _ _ H4 _ H3).
+        assert (exists mpmsg, mid_type (pmsg_mid mpmsg) = mty /\ In mpmsg (pmsgsOf impl1)).
+        { clear -i.
+          induction (pmsgsOf impl1); [inv i|].
+          inv i.
+          { exists a; split; intuition. }
+          { specialize (IHl H); dest.
+            eexists; repeat split; eauto.
+            right; auto.
+          }
+        }
+        destruct H6 as [mpmsg [? ?]].
+        specialize (Hmtdisj _ _ H7 H5).
+        rewrite H, H6 in Hmtdisj; auto.
+      
+    - right; intros.
+      pose proof (Himpl _ _ H0 H1).
+      destruct H2 as [obj [? [? ?]]].
+      apply in_app_or in H4; destruct H4.
+      + elim n; clear n.
+        pose proof (pmsgsOf_in _ _ H4 _ H3).
+        apply in_map with (f:= fun pmsg => mid_type (pmsg_mid pmsg)) in H5.
+        rewrite H in H5; assumption.
+      + exists obj; repeat split; assumption.
+  Qed.
+
+  Lemma atomic_steps_compositional:
+    forall ist1 hst ist2,
+      steps_det impl ist1 hst ist2 ->
+      forall tid min mouts,
+        Atomic impl tid min hst mouts ->
+        steps_det impl1 ist1 hst ist2 \/
+        steps_det impl2 ist1 hst ist2.
+  Proof.
+    intros.
+    pose proof (MTypeDisjSys_distr_same_type (mid_type (msg_id (tmsg_msg min)))).
+    pose proof (mtPreservineSys_atomic_same_msg_type Hmt H0 eq_refl H).
+    destruct H2 as [_ ?].
+    destruct H1.
+
+    - left.
+      clear -H H1 H2 Hii.
+      induction H; [constructor|].
+      inv H2.
+      specialize (IHsteps H6); clear H6.
+      econstructor; eauto; clear H IHsteps.
+      inv H0.
+      + constructor.
+      + constructor.
+        * unfold isExternal in *; rewrite <-Hii; assumption.
+        * unfold isInternal in *; rewrite <-Hii; assumption.
+      + simpl in H5, H9; rewrite H9 in H5.
+        specialize (H1 _ H5 _ H10 H).
+        destruct H1 as [obj1 [? [? ?]]].
+        replace (intOuts impl (toTMsgs nts (pmsg_outs fpmsg os (msg_value (getMsg fmsg)))))
+          with (intOuts impl1 (toTMsgs nts (pmsg_outs fpmsg os (msg_value (getMsg fmsg)))))
+          by (unfold intOuts, isInternal; rewrite Hii; reflexivity).
+        econstructor; eauto.
+        unfold isExternal in *; rewrite <-Hii; assumption.
+      + simpl in H5, H9; rewrite H9 in H5.
+        specialize (H1 _ H5 _ H10 H).
+        destruct H1 as [obj1 [? [? ?]]].
+        replace (intOuts impl (toTMsgs mts (pmsg_outs fpmsg os (msg_value (getMsg fmsg)))))
+          with (intOuts impl1 (toTMsgs mts (pmsg_outs fpmsg os (msg_value (getMsg fmsg)))))
+          by (unfold intOuts, isInternal; rewrite Hii; reflexivity).
+        econstructor; eauto.
+        unfold isInternal in *; rewrite <-Hii; assumption.
+
+    - right.
+      assert (indicesOf impl = indicesOf impl2) as Hii2 by (rewrite Hii; auto).
+      clear -H H1 H2 Hii2.
+      induction H; [constructor|].
+      inv H2.
+      specialize (IHsteps H6); clear H6.
+      econstructor; eauto; clear H IHsteps.
+      inv H0.
+      + constructor.
+      + constructor.
+        * unfold isExternal in *; rewrite <-Hii2; assumption.
+        * unfold isInternal in *; rewrite <-Hii2; assumption.
+      + simpl in H5, H9; rewrite H9 in H5.
+        specialize (H1 _ H5 _ H10 H).
+        destruct H1 as [obj1 [? [? ?]]].
+        replace (intOuts impl (toTMsgs nts (pmsg_outs fpmsg os (msg_value (getMsg fmsg)))))
+          with (intOuts impl2 (toTMsgs nts (pmsg_outs fpmsg os (msg_value (getMsg fmsg)))))
+          by (unfold intOuts, isInternal; rewrite Hii2; reflexivity).
+        econstructor; eauto.
+        unfold isExternal in *; rewrite <-Hii2; assumption.
+      + simpl in H5, H9; rewrite H9 in H5.
+        specialize (H1 _ H5 _ H10 H).
+        destruct H1 as [obj1 [? [? ?]]].
+        replace (intOuts impl (toTMsgs mts (pmsg_outs fpmsg os (msg_value (getMsg fmsg)))))
+          with (intOuts impl2 (toTMsgs mts (pmsg_outs fpmsg os (msg_value (getMsg fmsg)))))
+          by (unfold intOuts, isInternal; rewrite Hii2; reflexivity).
+        econstructor; eauto.
+        unfold isInternal in *; rewrite <-Hii2; assumption.
+  Qed.
   
+  Lemma transactional_steps_compositional:
+    forall ihst,
+      Transactional impl ihst ->
+      forall ist1 sst1,
+        ist1 ≈ sst1 ->
+        forall ist2,
+          steps_det impl ist1 ihst ist2 ->
+          exists (sst2 : TState) (shst : list TLabel),
+            map simP (behaviorOf impl ihst) = behaviorOf spec shst /\
+            steps_det spec sst1 shst sst2 /\ ist2 ≈ sst2.
+  Proof.
+    induction 1; simpl; intros; subst.
+
+    - inv H0; inv H4; inv H6.
+      exists sst1, nil; repeat split.
+      + constructor.
+      + assumption.
+
+    - assert (trsSteps impl1 ist1 (IlblIn (toTMsgU msg) :: nil) ist2).
+      { split; [|econstructor; reflexivity].
+        econstructor; [econstructor|].
+        inv H1; inv H4; inv H6.
+        eapply SdExt.
+        { unfold isExternal in *.
+          rewrite Hii in H1; assumption.
+        }
+        { unfold isInternal in *.
+          rewrite Hii in H3; assumption.
+        }
+      }
+      pose proof (Hsim1 H0 H).
+      simpl; simpl in H2; assumption.
+      
+    - pose proof (atomic_steps_compositional H1 H); destruct H2.
+      + assert (Transactional impl1 hst).
+        { econstructor.
+          eapply atomic_preserved; eauto.
+        }
+        pose proof (Hsim1 H0 (conj H2 H3)).
+        rewrite behaviorOf_preserved with (impl2:= impl1) by assumption.
+        assumption.
+      + assert (Transactional impl2 hst).
+        { econstructor.
+          eapply atomic_preserved; eauto.
+          rewrite Hii; assumption.
+        }
+        pose proof (Hsim2 H0 (conj H2 H3)).
+        rewrite behaviorOf_preserved with (impl2:= impl2) by (rewrite Hii; assumption).
+        assumption.
+  Qed.
+
+  Theorem trsSimulates_compositional: TrsSimulates simR simP impl spec.
+  Proof.
+    unfold TrsSimulates, trsSteps in *; intros.
+    destruct H0.
+    eapply transactional_steps_compositional; eauto.
+  Qed.
+
+End Compositionality.
+
